Some work on the proofs. Just realized the spec of inthash_insert_list needs to be changed, this commit saves the current work before modifications

verif_tuplekey/verif_inthash.v
@@ -1,50 +1,52 @@
 Require Import VST.floyd.proofauto.
 Require Import inthash.
 Require FMapWeakList.
+Require Import Program.Basics. Open Scope program_scope.
 Require Import Structures.OrdersEx.
 Instance CompSpecs : compspecs. make_compspecs prog. Defined.
 Definition Vprog : varspecs. mk_varspecs prog. Defined.
 
-Set Default Timeout 5. 
+Set Default Timeout 20. 
 Require Import VST.msl.iter_sepcon.
 Require Import VST.floyd.library.
 
-Definition V := { v: val | is_pointer_or_null v }.
+Definition V := sig is_pointer_or_null.
 Definition nullV: V := exist _ nullval mapsto_memory_block.is_pointer_or_null_nullval.
 Definition N: Z := 10.
 
 Module int_table := FMapWeakList.Make Z_as_DT.
+Print int_table.
 
 Section IntTable.
   Import int_table.
+  Check SetoidList.InA .
   Definition get_buckets (m: t V): list (list (Z*V)) :=
-    List.map (fun n => filter (fun '(k, v) => eq_dec (k mod N) (Z.of_nat n)) (elements m)) (seq 0%nat (Z.to_nat N)).
+    List.map (fun n => filter (fun kv => eq_dec (fst kv mod N) (Z.of_nat n)) (elements m)) (seq 0%nat (Z.to_nat N)).
 
   Lemma Zlength_get_buckets: forall m, Zlength (get_buckets m) = N.
   Proof.
     intros []. cbn.
     rewrite Zlength_map, Zlength_correct, seq_length. reflexivity.
   Qed.
-  
+
   Lemma get_buckets_spec (m: t V):
-    forall k v, MapsTo k v m <-> List.In (k, v) (Znth (k mod N) (get_buckets m)).
+    forall k v, MapsTo k v m <-> SetoidList.InA (eq_key_elt (elt := V)) (k, v) (Znth (k mod N) (get_buckets m)).
   Proof.
     intros.
     unshelve epose proof (Z_mod_lt k N _). unfold N. computable.
     assert (N = Zlength (seq 0%nat (Z.to_nat N))). rewrite Zlength_correct, seq_length. reflexivity.
     assert (mapsto_iff: MapsTo k v m <-> SetoidList.InA (@eq_key_elt _) (k, v) (elements m)).
     split; [apply elements_1 | apply elements_2].
-    rewrite mapsto_iff, SetoidList.InA_alt.
+    rewrite mapsto_iff.
     destruct m as [l nodup]. unfold get_buckets.
-    rewrite Znth_map, filter_In by omega.
+    rewrite Znth_map, SetoidList.filter_InA.
     rewrite <- nth_Znth by omega.
     rewrite seq_nth by now apply Z2Nat.inj_lt.
-    cbn. rewrite Z2Nat.id by omega. destruct initial_world.EqDec_Z.
-    { split.
-      + intros [[k' v'] [[] hin]].
-        cbn in *. now subst.
-      + intros [hin _]. exists (k, v). easy. }
-    contradiction.
+    cbn. rewrite Z2Nat.id by omega.
+    now destruct initial_world.EqDec_Z.
+    intros x y hxy. apply Raw.PX.eqke_eqk in hxy. now rewrite hxy.
+    rewrite Zlength_correct, seq_length, Z2Nat.id.
+    apply Z_mod_lt. unfold N; omega. unfold N; omega.
   Qed.
 
   Lemma MapsTo_inj: forall (m: t V) k v1 v2,
@@ -54,42 +56,57 @@ Section IntTable.
     apply find_1 in h1. apply find_1 in h2.
     rewrite h1 in h2. now inv h2.
   Qed.
+  
+  Lemma NoDupA_filter: forall (m: t V) (p: Z * V -> bool),
+      Proper (eq_key (elt := V) ==> eq) p ->
+ SetoidList.NoDupA (int_table.Raw.PX.eqk (elt:=V))
+    (filter p (int_table.elements (elt:=V) m)).
+  Proof.
+    intros [] p h.
+    induction this0.
+    constructor.
+    cbn. destruct p. constructor.
+    intros hcontr%SetoidList.filter_InA. now inversion NoDup0.
+    assumption.
+    unshelve eapply IHthis0. inversion NoDup0. assumption.
+    unshelve eapply IHthis0. inversion NoDup0. assumption.
+  Qed.
 End IntTable.
 
 Definition t_icell := Tstruct _icell noattr.
 Definition t_inthash := Tstruct _inthash noattr.
 
-Fixpoint icell_rep (sh: share) (l: list (Z*V)) (p: val): mpred :=
+Fixpoint icell_rep (l: list (Z*V)) (p: val): mpred :=
   match l with
   | [] => !!(p = nullval) && emp
   | (k, v) :: tl => EX q: val,
                     !! (0 <= k < Int.max_unsigned) &&
-                       malloc_token sh t_icell p *
-                    data_at sh t_icell (Vint (Int.repr k), (proj1_sig v, q)) p *
-                    icell_rep sh tl q
+                       malloc_token Ews t_icell p *
+                    data_at Ews t_icell (Vint (Int.repr k), (proj1_sig v, q)) p *
+                    icell_rep tl q
   end.
 
 Definition icell_rep_local_facts:
-  forall sh l p, icell_rep sh l p |-- !! (is_pointer_or_null p /\ (p=nullval <-> l = [])).
+  forall l p, icell_rep l p |-- !! (is_pointer_or_null p /\ (p=nullval <-> l = [])).
 Proof.
-  intros sh l. induction l as [ | [] tl]; intro p; simpl.
+  intros l. induction l as [ | [] tl]; intro p; simpl.
   + entailer!. easy.
   + Intros q. entailer!. now apply field_compatible_nullval1 in H1.
 Qed.
 Hint Resolve icell_rep_local_facts: saturate_local.
 
 Definition icell_rep_valid_pointer:
-  forall sh l p, readable_share sh -> icell_rep sh l p |-- valid_pointer p.
-Proof. intros sh [|[]] p h; cbn; entailer. Qed.
+  forall l p, icell_rep l p |-- valid_pointer p.
+Proof. intros [|[]] p; cbn; entailer. Qed.
 Hint Resolve icell_rep_valid_pointer: valid_pointer.
 
-Definition inthash_rep (sh: share) (m: int_table.t V) (p: val): mpred :=
+Definition inthash_rep (m: int_table.t V) (p: val): mpred :=
   let buckets := get_buckets m in
   EX buckets_p: list val,
   !! (Zlength buckets_p = N) &&
-     malloc_token sh t_inthash p *
-  data_at sh t_inthash buckets_p p *
-  iter_sepcon (prod_curry (icell_rep sh)) (combine buckets buckets_p).
+     malloc_token Ews t_inthash p *
+  data_at Ews t_inthash buckets_p p *
+  iter_sepcon (prod_curry icell_rep) (combine buckets buckets_p).
 
 Definition inthash_new_spec: ident * funspec :=
    DECLARE _inthash_new
@@ -102,7 +119,7 @@ Definition inthash_new_spec: ident * funspec :=
    EX p:val,
       PROP() 
       LOCAL(temp ret_temp p) 
-      SEP(inthash_rep Ews (int_table.empty V) p; mem_mgr gv).
+      SEP(inthash_rep (int_table.empty V) p; mem_mgr gv).
 
 Definition new_icell_spec: ident * funspec :=
    DECLARE _new_icell
@@ -110,12 +127,12 @@ Definition new_icell_spec: ident * funspec :=
  PRE [ _key OF tuint, _value OF tptr tvoid, _next OF tptr t_icell ] 
    PROP( 0 <= key < Int.max_unsigned )
    LOCAL(gvars gv; temp _key (Vint (Int.repr key)); temp _value (proj1_sig value); temp _next pnext)
-   SEP(icell_rep Ews tl pnext; mem_mgr gv)
+   SEP(icell_rep tl pnext; mem_mgr gv)
  POST [ tptr t_icell ] 
    EX p:val,
       PROP() 
       LOCAL(temp ret_temp p) 
-      SEP(icell_rep Ews ((key, value) :: tl) p; mem_mgr gv).
+      SEP(icell_rep ((key, value) :: tl) p; mem_mgr gv).
 
 Definition inthash_lookup_spec: ident * funspec :=
    DECLARE _inthash_lookup
@@ -123,15 +140,14 @@ Definition inthash_lookup_spec: ident * funspec :=
  PRE [ _p OF tptr t_inthash, _key OF tuint ] 
    PROP(0 <= key < Int.max_unsigned)
    LOCAL(gvars gv; temp _p pm; temp _key (Vint (Int.repr key)))
-   SEP(mem_mgr gv; inthash_rep Ews m pm)
+   SEP(mem_mgr gv; inthash_rep m pm)
  POST [ tptr tvoid ] 
-   EX p:val,
-      PROP(match int_table.find key m with
-             | Some res => p = proj1_sig res
-             | None => p = Vnullptr
-          end) 
-      LOCAL(temp ret_temp p) 
-      SEP(mem_mgr gv; inthash_rep Ews m pm).
+      PROP() 
+      LOCAL(temp ret_temp (match int_table.find key m with
+             | Some res => proj1_sig res
+             | None => Vnullptr
+          end)) 
+      SEP(mem_mgr gv; inthash_rep m pm).
 
 Definition inthash_insert_list_spec: ident * funspec :=
    DECLARE _inthash_insert_list
@@ -139,94 +155,308 @@ Definition inthash_insert_list_spec: ident * funspec :=
  PRE [ _r0 OF tptr (tptr t_icell), _key OF tuint ] 
    PROP(0 <= key < Int.max_unsigned; SetoidList.NoDupA (int_table.Raw.PX.eqk (elt:=V)) l)
    LOCAL(gvars gv; temp _r0 ppl; temp _key (Vint (Int.repr key)))
-   SEP(mem_mgr gv; data_at Ews (tptr t_icell) pl ppl; icell_rep Ews l pl)
+   SEP(mem_mgr gv; data_at Ews (tptr t_icell) pl ppl; icell_rep l pl)
  POST [ tptr t_icell ] 
-   EX p_ret: val, EX v: V, EX r: val, EX tl: list (Z * V),
+   EX p_ret: val, EX r: val, EX pre tl: list (Z * V), EX v: V,
       let new_l := if int_table.Raw.mem key l then l else l ++ [(key, nullV)] in
-      PROP( )
+      PROP( new_l = pre ++ (key, v) :: tl )
       LOCAL(temp ret_temp p_ret) 
-      SEP(mem_mgr gv; data_at Ews (tptr t_icell) p_ret r; icell_rep Ews ((key, v) :: tl) p_ret;
-          (data_at Ews (tptr t_icell) p_ret r * icell_rep Ews ((key, v) :: tl) p_ret) -* (EX p: val, data_at Ews (tptr t_icell) p ppl * icell_rep Ews new_l p)).
+      SEP(mem_mgr gv; data_at Ews (tptr t_icell) p_ret r * icell_rep ((key, v) :: tl) p_ret;
+          data_at Ews (tptr t_icell) p_ret r * icell_rep ((key, v) :: tl) p_ret -*
+          EX pl: val, data_at Ews (tptr t_icell) pl ppl * icell_rep new_l pl).
+
+Definition inthash_insert_spec: ident * funspec :=
+   DECLARE _inthash_insert
+ WITH gv: globals, m: int_table.t V, key: Z, pm: val, v: V
+ PRE [ _p OF tptr t_inthash, _key OF tuint, _value OF tptr tvoid ] 
+   PROP(0 <= key < Int.max_unsigned)
+   LOCAL(gvars gv; temp _p pm; temp _key (Vint (Int.repr key)); temp _value (proj1_sig v))
+   SEP(mem_mgr gv; inthash_rep m pm)
+ POST [ tptr tvoid ] 
+      PROP( ) 
+      LOCAL(temp ret_temp (match int_table.find key m with Some v => proj1_sig v | None => nullval end)) 
+      SEP(mem_mgr gv; inthash_rep (int_table.add key v m) pm).
 
 Definition Gprog : funspecs :=
         ltac:(with_library prog [ inthash_new_spec; new_icell_spec; inthash_lookup_spec ;
-             inthash_insert_list_spec ]).
+             inthash_insert_list_spec ; inthash_insert_spec ]).
+
+Lemma focus_bucket (m: int_table.t V) (key: Z) (buckets_p: list val)
+      (h: Zlength buckets_p = N):
+  let l := combine (get_buckets m) buckets_p in
+  let i := key mod N in
+  iter_sepcon (prod_curry icell_rep) l =
+  iter_sepcon (prod_curry icell_rep) (sublist 0 i l) *
+  (icell_rep (Znth i (get_buckets m)) (Znth i buckets_p) *
+   iter_sepcon (prod_curry icell_rep) (sublist (i + 1) N l)).
+Proof.
+  intros l i.
+  assert (0 <= i < N). { apply Z_mod_lt. unfold N. omega. }
+  assert (Zlength l = N).
+  { unfold l. rewrite Zlength_correct, combine_length.
+    rewrite Min.min_l, <- Zlength_correct. apply Zlength_get_buckets.
+    apply Nat2Z.inj_le. rewrite <- Zlength_correct, <- Zlength_correct, Zlength_get_buckets. omega. }
+  replace l with (sublist 0 i l ++ [(Znth i (get_buckets m), Znth i buckets_p)]
+                          ++ sublist (i+1) N l) at 1.
+  do 2 rewrite iter_sepcon_app.
+  simpl iter_sepcon. rewrite sepcon_emp. reflexivity.
+  symmetry.
+  erewrite <- sublist_same at 1.
+  erewrite sublist_split at 1. f_equal.
+  erewrite sublist_split at 1. erewrite sublist_len_1 at 1.
+  unfold l. rewrite <- nth_Znth, combine_nth, nth_Znth, nth_Znth. reflexivity.
+  omega.
+  rewrite Zlength_get_buckets. assumption.
+  apply Nat2Z.inj. rewrite <- Zlength_correct, <- Zlength_correct, Zlength_get_buckets. congruence.
+  fold l. omega. omega. omega. omega. omega. omega. omega. symmetry. assumption.
+Qed.
 
 Lemma body_inthash_insert_list: semax_body Vprog Gprog f_inthash_insert_list inthash_insert_list_spec.
 Proof.
   start_function.
-  forward.
-  Let icell_box_rep l r := EX p: val, data_at Ews (tptr t_icell) p r * icell_rep Ews l p.
+  forward. Search data_at Vundef.
   forward_loop
     (EX l1 l2: list (Z * V), EX r: val,
       PROP ( l = l1 ++ l2; not (int_table.Raw.PX.In key l1) )
      LOCAL (temp _r r; gvars gv; temp _r0 ppl; temp _key (Vint (Int.repr key)))
-     SEP (mem_mgr gv; icell_box_rep l2 r; ALL l', icell_box_rep l' r -* icell_box_rep (l1 ++ l') ppl)).
-  + Exists (@nil (Z*V)) l ppl.
+     SEP (mem_mgr gv;
+          EX p: val, data_at Ews (tptr t_icell) p r * icell_rep l2 p;
+          ALL l', (EX p, data_at Ews (tptr t_icell) p r * icell_rep l' p) -* EX pl: val, data_at Ews (tptr t_icell) pl ppl * icell_rep (l1 ++ l') pl)).
+  + Exists (@nil (Z*V)) l ppl pl.
     entailer!. destruct H4 as [x hx]. inversion hx.
-    unfold icell_box_rep.
-    Exists pl. cancel. apply allp_right. intro. apply wand_refl_cancel_right.
-  + Intros l1 l2 r.
-    unfold icell_box_rep at 1. Intros p.
+    apply allp_right. intro.
+    apply wand_refl_cancel_right.
+  + Intros l1 l2 r p.
     forward.
     forward_if.
   - forward_call (gv, key, nullV, nullval, @nil (Z*V)).
     cbn. entailer!.
-    Intros vret.
+    Intro vret.
     do 2 forward.
     replace l2 with (@nil (Z*V)) by intuition. rewrite app_nil_r.
     replace (int_table.Raw.mem (elt := V) key l1) with false.
-    Exists vret nullV r (@nil (Z*V)). cancel. unfold icell_rep at 1 2 3 4. entailer. 
-    sep_apply (allp_instantiate (fun l' => icell_box_rep l' r -* icell_box_rep (l1 ++ l') ppl) [(key, nullV)]).
-    Exists nullval. entailer!.
-    rewrite <- wand_sepcon_adjoint. Intros q. subst q.
-    rewrite sepcon_assoc, sepcon_comm.
-    eapply derives_trans. eapply modus_ponens_wand'.
-    unfold icell_box_rep, icell_rep. Exists vret. cancel. Exists nullval. entailer!.
-    unfold icell_box_rep. apply derives_refl.
+    Exists vret r l1 (@nil (Z*V)) nullV.
+    sep_apply (allp_instantiate (fun l' =>
+                                   (EX p0 : val, data_at Ews (tptr t_icell) p0 r * icell_rep l' p0) -*
+   (EX pl0 : val, data_at Ews (tptr t_icell) pl0 ppl * icell_rep (l1 ++ l') pl0)) [(key, nullV)]).
+    unfold icell_rep at 4.
+    entailer!.
+    apply wand_derives. Exists vret. apply derives_refl.
+    apply derives_refl.
     symmetry. apply not_true_is_false.
     intro h.
     unshelve eapply (int_table.Raw.mem_2 _) in h. clear -H0.
     induction l2. rewrite <- app_nil_r. assumption.
     apply IHl2. eapply SetoidList.NoDupA_split. exact H0.
     contradiction.
-  - destruct l2 as [|[]]. unfold icell_rep. Intros. contradiction.
+  - destruct l2 as [|[k v]]. unfold icell_rep. Intros. contradiction.
     unfold icell_rep; fold icell_rep. Intros q.    
     forward. forward_if.
     ++ forward.
        replace (int_table.Raw.mem (elt:=V) key (l1 ++ (key, v) :: l2)) with true.
-       Exists p v r l2.
-       sep_apply (allp_instantiate (fun l' => icell_box_rep l' r -* icell_box_rep (l1 ++ l') ppl) ((key, v)::l2)).
-       cbn.
-       entailer!. Exists q.
-       cancel. 
-       apply wand_derives.
-       { Intro pnext. unfold icell_box_rep. Exists p. cbn. Exists pnext.
-         entailer!. }
-       { apply derives_refl. }
+       Exists p r l1 l2 v.
+       sep_apply (allp_instantiate (fun l' =>
+   (EX p0 : reptype (tptr t_icell), data_at Ews (tptr t_icell) p0 r * icell_rep l' p0) -*
+   (EX pl0 : val, data_at Ews (tptr t_icell) pl0 ppl * icell_rep (l1 ++ l') pl0)) ((key, v)::l2)).
+       unfold icell_rep at 4; fold icell_rep. Exists q.
+       entailer!.
+       apply wand_derives. Exists p. apply derives_refl.
+       apply derives_refl.
        symmetry. apply int_table.Raw.mem_1. assumption.
        rewrite int_table.Raw.PX.In_alt. exists v.
        rewrite SetoidList.InA_app_iff. right. constructor. constructor.
-    ++ forward. unfold_data_at (data_at _ _ _ p).
-       rewrite (field_at_data_at _ _ [StructField _next]).
-       Exists (l1 ++ [(z,v)]) l2 (field_address t_icell [StructField _next] p).
-       entailer!. split. now rewrite <- app_assoc.
-       { clear -H2 H5. rewrite int_table.Raw.PX.In_alt in H2 |- *. intros [v' hv'].
-         rewrite SetoidList.InA_app_iff in hv'. destruct hv'.
-         apply H2. exists v'. assumption.
-         inversion H. inversion H1. cbn in H4. now subst.
-         inversion H1. }
-       unfold icell_box_rep at 3. Exists q.
-       cancel. apply allp_right. intro l3. rewrite <- app_assoc. cbn.
-       sep_apply (allp_instantiate (fun l' => icell_box_rep l' r -* icell_box_rep (l1 ++ l') ppl) ((z, v)::l3)).
-       rewrite <- wand_sepcon_adjoint, sepcon_assoc, sepcon_comm.
-       apply wand_frame_elim'.
-       unfold icell_box_rep. Exists p. cbn.
-       Intro p0.
-       Exists p0.
-       unfold_data_at (data_at _ _ _ p). rewrite (field_at_data_at _ _ [StructField _next]).
+    ++ forward.
+       Exists (l1 ++ [(k,v)]) l2 (offset_val
+              (align (align (align 0 (alignof tuint) + sizeof tuint) (alignof (tptr tvoid)) + sizeof (tptr tvoid))
+                 (alignof (tptr (Tstruct _icell noattr)))) p).
        entailer!.
+       { split. now rewrite <- app_assoc.
+         rewrite int_table.Raw.PX.In_alt in H2 |- *. intros [v' hv'].
+         rewrite SetoidList.InA_app_iff in hv'. destruct hv' as [hv' | hv'].
+         apply H2. exists v'. assumption.
+         apply SetoidList.InA_singleton in hv'.
+         compute in hv'. congruence.
+       }
+       Exists q.
+       unfold_data_at (data_at _ _ _ p).
+       rewrite (field_at_data_at _ _ [StructField _next]).
+       rewrite field_address_offset. cbn.
+       cancel. apply allp_right.
+       intro l3.
+       sep_apply (allp_instantiate (fun l' =>
+   (EX p0 : val, data_at Ews (tptr t_icell) p0 r * icell_rep l' p0) -*
+   (EX pl0 : val, data_at Ews (tptr t_icell) pl0 ppl * icell_rep (l1 ++ l') pl0)) ((k, v)::l3)).
+       rewrite <- wand_sepcon_adjoint.
+       Intro p0.
+       rewrite sepcon_assoc, sepcon_comm.
+       sep_apply ( wand_frame_elim' (data_at Ews (tptr t_icell) p r *
+  (malloc_token Ews t_icell p *
+   (field_at Ews t_icell [StructField _key] (Vint (Int.repr k)) p *
+    field_at Ews t_icell [StructField _value] (proj1_sig v) p)) *
+  (data_at Ews (tptr t_icell) p0 (offset_val 8 p) * icell_rep l3 p0))).
+       Exists p. cbn. Exists p0.
+       unfold_data_at (data_at _ _ _ p).
+       rewrite (field_at_data_at _ _ [StructField _next]).
+       rewrite field_address_offset. entailer!. auto with field_compatible.
+       rewrite <- app_assoc. apply derives_refl.
+       auto with field_compatible.
 Qed.
+
+Lemma body_inthash_insert: semax_body Vprog Gprog f_inthash_insert inthash_insert_spec.
+Proof.
+  start_function.
+  unfold inthash_rep. Intros buckets_p.
+  rewrite focus_bucket with (key := key).
+  Intros.
+  unfold_data_at (data_at _ _ _ pm).
+  rewrite field_at_data_at'. simpl nested_field_type. fold t_icell.
+  pose (i := key mod N).
+  assert (h_i: 0 <= i < N). apply Z_mod_lt. unfold N. omega.
+  rewrite wand_slice_array with (lo := i) (hi := i + 1).
+  replace (i+1-i) with 1 by omega.
+  rewrite sublist_len_1.
+  erewrite data_at_singleton_array_eq by reflexivity.
+  forward_call (gv, Znth i (get_buckets m), key,  (field_address0 (tarray (tptr t_icell) 10) [ArraySubsc i]
+           (offset_val (nested_field_offset t_inthash [StructField _buckets]) pm)), Znth i buckets_p).
+  entailer!.
+  rewrite field_address0_offset. simpl nested_field_offset.
+  rewrite Z.add_0_l. reflexivity.
+  eapply field_compatible0_cons_Tarray. reflexivity. auto.
+  fold N. unfold i. unshelve epose proof (Z_mod_lt key N _). unfold N. omega. omega.
+  instantiate (Frame := [malloc_token Ews t_inthash pm; array_with_hole Ews (tptr t_icell) i (i + 1) 10 buckets_p pm;
+  iter_sepcon (prod_curry icell_rep) (sublist 0 (key mod N) (combine (get_buckets m) buckets_p));
+  iter_sepcon (prod_curry icell_rep)
+    (sublist (key mod N + 1) N (combine (get_buckets m) buckets_p))]). unfold Frame. unfold fold_right_sepcon, i. entailer!.
+  split. assumption.
+  unfold get_buckets. rewrite Znth_map.
+  apply NoDupA_filter.
+  { intros x y ->. reflexivity. }
+  { rewrite Zlength_correct, seq_length. rep_omega. }
+  Intros vret.
+  destruct vret as [[[[p_ret r] pre] tl] [old_v holdv]]. unfold fst, snd in *.
+  unfold icell_rep at 1; fold icell_rep. Intros q.
+  do 3 forward.
+  {
+    entailer!.
+    { rename H1 into h. clear -h h_i.
+      pose (l := Znth i (get_buckets m)). fold l in h.
+      case_eq (int_table.Raw.mem (elt := V) key l); intro hmem; rewrite hmem in h.
+      -- assert (hmapsto: int_table.MapsTo key (exist _ old_v holdv: V) m).
+         { unfold l in h. rewrite get_buckets_spec.
+           fold i. rewrite h.
+           rewrite SetoidList.InA_app_iff. right. constructor. reflexivity. }
+         rewrite (int_table.find_1 hmapsto). reflexivity.
+      -- assert (hin: not (int_table.Raw.PX.In (elt := V) key l)).
+         { intro hcontr. apply int_table.Raw.mem_1 in hcontr. congruence.
+           unfold l, get_buckets. rewrite Znth_map.
+           apply NoDupA_filter. now intros x y ->.
+           rewrite Zlength_correct, seq_length. rep_omega. }
+
+         case_eq (int_table.find (elt := V) key m).
+         +++ intros v0 hv0%int_table.find_2%get_buckets_spec.
+         rewrite int_table.Raw.PX.In_alt in hin.
+         exfalso. apply hin. exists v0. now apply int_table.Raw.PX.InA_eqke_eqk.
+         
+         +++ intro hnone.
+             destruct tl. apply app_inj_tail in h.
+             destruct h as [_ h]. now inversion h.
+             exfalso.
+             clear hmem.
+             revert pre h hin.
+             induction l; intros pre h hin.
+             --- apply (f_equal (@length _)) in h.
+                 rewrite app_length, app_length in h. cbn in h. omega.
+             --- destruct pre.
+                 cbn in h. inversion h. apply hin. rewrite int_table.Raw.PX.In_alt.
+                 exists (exist is_pointer_or_null old_v holdv). constructor. congruence.
+                 eapply IHl. do 2 rewrite <- app_comm_cons in h. inversion h. eassumption.
+                 intro hcontr. apply hin. rewrite int_table.Raw.PX.In_alt in hcontr |- *.
+                 destruct hcontr as [e he]. exists e. now apply SetoidList.InA_cons_tl. }
+    
+    entailer.
+    
+    unfold inthash_rep.
+    
+
+    Exists (sublist 0 i buckets_p ++ pl :: sublist (i + 1) N buckets_p).
+      
+      
+ }
+
+  cbn; omega.
+  omega.
+  fold N; omega.
+  fold N; assumption.
+  assumption.
+Admitted.
+
+
+  { unfold inthash_rep. Exists buckets_p. entailer!.
+    { 
+      case_eq (int_table.Raw.mem key (Znth i (get_buckets m))).
+      + intro hmem.
+        rewrite hmem in H2.
+        apply int_table.Raw.mem_2 in hmem.
+        rewrite int_table.Raw.PX.In_alt in hmem. destruct hmem as [v_ hv_].
+        rewrite SetoidList.InA_alt in hv_.
+        destruct hv_ as [[yn yv] [hyeq hyin]].
+        unfold int_table.Raw.PX.eqk in hyeq. cbn in hyeq.
+        unfold i in hyin. rewrite <- hyeq, <- get_buckets_spec in hyin.
+        assert (hmapsto2: int_table.MapsTo key (exist _ v0 hv0) m).
+        { rewrite get_buckets_spec. fold i. rewrite H2.
+          apply in_or_app. right. constructor. reflexivity. }
+        pose proof (MapsTo_inj _ _ _ _ hyin hmapsto2).
+        apply int_table.find_1 in hyin. rewrite hyin.
+        subst. reflexivity.
+        unfold get_buckets. rewrite Znth_map.
+        apply (NoDupA_filter m (fun z => eq_dec (z mod N) _)).
+        rewrite Zlength_correct, seq_length, Z2Nat.id. assumption.
+        omega.
+      + intro hmem.
+        rewrite hmem in H2.
+        admit. }
+    rewrite focus_bucket with (key := key) by assumption.
+    entailer!.
+    sep_apply (modus_ponens_wand' (data_at Ews (tptr t_icell) p_ret r * malloc_token Ews t_icell p_ret *
+  data_at Ews t_icell (Vint (Int.repr key), (proj1_sig v, q)) p_ret * icell_rep tl q)).
+    unfold icell_rep; fold icell_rep. Exists q. entailer!.
+    unfold_data_at (data_at _ _ _ pm).
+    rewrite field_at_data_at'. simpl nested_field_type. fold t_icell.
+    rewrite wand_slice_array with (lo := i) (hi := i + 1).
+    replace (i+1-i) with 1 by omega.
+    rewrite sublist_len_1.
+    erewrite data_at_singleton_array_eq by reflexivity.
+    simpl nested_field_offset. rewrite isptr_offset_val_zero. entailer!.
+    rewrite sepcon_assoc.
+    sep_apply modus_ponens_wand'. entailer!.
+    sep_apply modus_ponens_wand'.
+    replace (iter_sepcon (prod_curry icell_rep)
+        (sublist 0 (key mod N) (combine (get_buckets (int_table.add key v m)) buckets_p)))
+            with
+               (iter_sepcon (prod_curry icell_rep) (sublist 0 (key mod N) (combine (get_buckets m) buckets_p))).
+    replace (iter_sepcon (prod_curry icell_rep)
+        (sublist (key mod N + 1) (Zlength (combine (get_buckets (int_table.add key v m)) buckets_p))
+           (combine (get_buckets (int_table.add key v m)) buckets_p))) with
+        (iter_sepcon (prod_curry icell_rep)
+     (sublist (key mod N + 1) (Zlength (combine (get_buckets m) buckets_p)) (combine (get_buckets m) buckets_p))). cancel.
+    replace (Znth (key mod N) (get_buckets (int_table.add key v m))) with
+        (if int_table.Raw.mem (elt:=V) key (Znth i (get_buckets m))
+     then Znth i (get_buckets m)
+     else Znth i (get_buckets m) ++ [(key, nullV)]).
+    apply derives_refl.
+    admit.
+    admit.
+    admit.
+    admit.
+    admit.
+    admit.
+    admit.
+    admit.
+  }
+  unfold reptype, reptype_gen. cbn. rewrite H0. assumption. 
+  omega. fold N. omega.
+  fold N. assumption. assumption.
+Admitted.
 
 Lemma body_inthash_lookup: semax_body Vprog Gprog f_inthash_lookup inthash_lookup_spec.
 Proof.
@@ -235,7 +465,7 @@ Proof.
   Intros buckets_p.
   remember (combine (get_buckets m) buckets_p) as l.
   remember (key mod N) as i.
-  remember (iter_sepcon (prod_curry (icell_rep Ews)) l) as buckets_rep eqn:hb.
+  remember (iter_sepcon (prod_curry icell_rep) l) as buckets_rep eqn:hb.
   pose proof hb as save_buckets_rep.
   replace l with (sublist 0 i l ++ [(Znth i (get_buckets m), Znth i buckets_p)]
                           ++ sublist (i+1) (Zlength l) l) in hb.
@@ -253,15 +483,18 @@ Proof.
     remember (Znth i (get_buckets m)) as kvs.
     forward_while (
         EX kvs1 kvs2: list (Z * V), EX q: val,
-     PROP ( kvs = kvs1 ++ kvs2 /\ Forall (fun '(k, v) => k <> key) kvs1)
+     PROP ( kvs = kvs1 ++ kvs2 /\ not (int_table.Raw.PX.In key kvs1))
      LOCAL (temp _q q; gvars gv; temp _p pm; temp _key (Vint (Int.repr key)))
      SEP (mem_mgr gv; malloc_token Ews t_inthash pm; data_at Ews t_inthash buckets_p pm;
-     iter_sepcon (prod_curry (icell_rep Ews)) (sublist 0 i l);
-     icell_rep Ews kvs2 q;
-     icell_rep Ews kvs2 q -* icell_rep Ews kvs q0;
-     emp; iter_sepcon (prod_curry (icell_rep Ews)) (sublist (i + 1) (Zlength l) l)))%assert.
-    + Exists (@nil (Z*V)). Exists kvs. Exists q0.
-      entailer!. apply wand_refl_cancel_right.
+     iter_sepcon (prod_curry icell_rep) (sublist 0 i l);
+     icell_rep kvs2 q;
+     icell_rep kvs2 q -* icell_rep kvs q0;
+     emp; iter_sepcon (prod_curry icell_rep) (sublist (i + 1) (Zlength l) l)))%assert.
+    + Exists (@nil (Z*V)) kvs q0.
+      entailer!.
+      { rewrite int_table.Raw.PX.In_alt in H5. destruct H5 as [e he].
+        inv he. }      
+      apply wand_refl_cancel_right.
     + entailer!.
     + destruct kvs2. assert_PROP (q = nullval). entailer!. intuition.
       subst q. contradiction.
@@ -273,7 +506,6 @@ Proof.
         destruct v as [v hv].
         forward.
         forward.
-        Exists v.
         replace (int_table.find key m) with (Some v_sig).
         entailer!.
         unfold inthash_rep. Exists buckets_p.
@@ -282,17 +514,23 @@ Proof.
         eapply modus_ponens_wand'. unfold icell_rep at 2; fold icell_rep.
         Exists q1. entailer. 
         symmetry. eapply int_table.find_1. rewrite get_buckets_spec.
-        rewrite (proj1 H1). apply in_or_app. right. constructor. reflexivity.
+        rewrite (proj1 H1), SetoidList.InA_app_iff. right. constructor. reflexivity.
       - forward. Exists (kvs1 ++ [(k,v)], kvs2, q1).
         entailer!.
         destruct H1. split.
         rewrite <- app_assoc. unfold app at 2. assumption.
-        rewrite Forall_app. split. assumption. constructor. assumption. constructor.
+        { intro hcontr.
+          rewrite int_table.Raw.PX.In_alt in hcontr, H11.
+          destruct hcontr as [e he].
+          rewrite SetoidList.InA_app_iff in he. destruct he as [he|he].
+          apply H11. exists e. assumption.
+          rewrite SetoidList.InA_singleton in he.
+          compute in he. subst. contradiction. }
         cancel. rewrite <- wand_sepcon_adjoint.
         rewrite sepcon_comm, <- sepcon_assoc.
         apply modus_ponens_wand'. unfold icell_rep at 2; fold icell_rep.
         Exists q1. entailer!.
-      + forward. Exists Vnullptr.
+      + forward.
         replace (int_table.find (elt := V) key m) with (@None V).
         unfold inthash_rep. Exists buckets_p.
         rewrite <- save_buckets_rep. entailer!. apply modus_ponens_wand.
@@ -301,9 +539,12 @@ Proof.
         remember (int_table.find (elt := V) key m) as f. destruct f.
         symmetry in Heqf. apply int_table.find_2 in Heqf.
         rewrite get_buckets_spec in Heqf.
-        destruct H1 as [hnth hforall].
-        rewrite hnth in Heqf. rewrite Forall_forall in hforall.
-        apply hforall in Heqf. contradiction. reflexivity.
+        destruct H1 as [hnth hnin].
+        rewrite hnth in Heqf.
+        exfalso. apply hnin.
+        rewrite int_table.Raw.PX.In_alt.
+        exists v. apply int_table.Raw.PX.InA_eqke_eqk. assumption.
+        reflexivity.
   }
   assert (hlenl: Zlength l = N).
   { subst l. rewrite Zlength_correct, combine_length, Min.min_l, <- Zlength_correct, Zlength_get_buckets.
@@ -386,7 +627,7 @@ Proof.
      LOCAL (temp _p vret; gvars gv; temp _key (Vint (Int.repr key)); temp _value (proj1_sig value);
      temp _next pnext)
      SEP (mem_mgr gv; malloc_token Ews t_icell vret * data_at_ Ews t_icell vret;
-     icell_rep Ews tl pnext)).
+     icell_rep tl pnext)).
   + destruct eq_dec; entailer.
   + forward_call tt. contradiction.
   + forward. rewrite if_false by assumption. entailer.
